Managed to get the definition command for CML implicit functions working!

theories/models/utp_cml/utp_cml_commands.thy
@@ -12,28 +12,62 @@ imports
 keywords "cmlifun" :: thy_decl and "inps" "outs" "pre" "post"
 begin
 
+abbreviation "swap \<equiv> \<lambda> (x,y). (y, x)"
 
+definition mk_ifun_body :: "'a set \<Rightarrow> 'b set \<Rightarrow> ('a \<Rightarrow> bool cmle) \<Rightarrow> (('a * 'b) \<Rightarrow> bool cmle) \<Rightarrow> ('a * 'b) set" where
+"mk_ifun_body A B pre post 
+  = {(x,y) | x y. x \<in> A \<and> y \<in> B \<and> \<lbrakk>pre(x)\<rbrakk>\<^sub>*\<B> = Some True \<and> \<lbrakk>post(x,y)\<rbrakk>\<^sub>*\<B> = Some True}"
 
-ML {* 
-foldr1 (fn (x,y) => Syntax.const (unprefix "\<^const>" @{const_syntax vty_prod}) $ x $ y);
+ML {*
+local
+  fun absnm' x n (u $ t) = (absnm' x n u) $ (absnm' x n t)
+    | absnm' x n (Free (y, t)) = if (x = y) then Bound n else Free (y, t)
+    | absnm' x n (Abs (y, ty, tr)) = if (x = y) then (Abs (y, ty, tr)) else (Abs (y, ty, absnm' x n tr))
+    | absnm' _ _ e = e;
+in fun absnm (x, ty) n tr = Abs (x, ty, absnm' x n tr) end;
 
+fun get_cml_holty ty ctxt =
+  let val tctxt = (Config.put Syntax.root @{nonterminal "vty"} ctxt) in
+  case (type_of (Syntax.read_term tctxt ty)) of
+    Type (_, [ty]) => ty
+  | x => error (@{make_string} x)
+ end;
+
+local
+  fun mk_lambda' [(id, ty)] n term ctxt =
+        absnm (id, get_cml_holty ty ctxt) n term
+    | mk_lambda' ((id, ty) :: xs) n term ctxt =
+        Const (@{const_name "prod_case"}, dummyT) $ absnm (id, get_cml_holty ty ctxt) n (mk_lambda' xs (n - 1) term ctxt)
+    | mk_lambda' [] _ term _ = term;
+in
+  fun mk_lambda xs term ctxt = mk_lambda' xs (length xs - 1) term ctxt
+end;
 
 fun mk_fun ((id, (inp, out)), (pre, post)) ctxt = 
-  let val pctxt = (Config.put Syntax.root (unprefix "\<^type>" @{type_syntax "n_pexpr"}) ctxt)
-      val tctxt = (Config.put Syntax.root (unprefix "\<^type>" @{type_syntax "vty"}) ctxt)
+  let val pctxt = (Config.put Syntax.root @{nonterminal "n_pexpr"} ctxt)
+      val tctxt = (Config.put Syntax.root @{nonterminal "vty"} ctxt)
       val preb = (Binding.name ("pre_" ^ id), NoSyn)
-      val preb_def = ( (Binding.name ("pre_" ^ id ^ "_def"), [])
-                     , Syntax.read_term pctxt pre)
+      val preb_term = Syntax.check_term pctxt (mk_lambda inp (Syntax.parse_term pctxt pre) ctxt)
+      val preb_type = type_of preb_term
+      val preb_def = ( (Binding.name ("pre_" ^ id ^ "_def"), []), preb_term)
       val postb = (Binding.name ("post_" ^ id), NoSyn)
-      val postb_def = ( (Binding.name ("post_" ^ id ^ "_def"), [])
-                      , Syntax.read_term pctxt post)
-      val inpt = (Binding.name ("inp_" ^ id), NoSyn)
-      val inpt_def = ( (Binding.name ("inp_" ^ id ^ "_def"), [])
-                     , foldr1 (fn (x,y) => @{term "vty_prod"} $ x $ y) (map (Syntax.read_term tctxt o snd) inp))
-  in
-    ((Local_Theory.define (preb, preb_def) #> snd) o 
-     (Local_Theory.define (postb, postb_def) #> snd) o
-     (Local_Theory.define (inpt, inpt_def) #> snd)) ctxt
+      val postb_term = (Syntax.check_term pctxt 
+                          (Const (@{const_name "comp"}, dummyT) 
+                            $ (mk_lambda (out :: inp) (Syntax.parse_term pctxt post) ctxt)
+                            $ Const (@{const_abbrev "swap"}, dummyT)))
+      val postb_def = ( (Binding.name ("post_" ^ id ^ "_def"), []), postb_term) 
+      val inpt = foldr1 (fn (x,y) => 
+            (Syntax.check_term ctxt (Syntax.const @{const_abbrev "vty_prod"} $ x $ y)))
+                                     (map (Syntax.read_term tctxt o snd) inp)
+      val outt = Syntax.read_term tctxt (snd out)
+      val ppctxt = ((Local_Theory.define (preb, preb_def) #> snd) o
+                    (Local_Theory.define (postb, postb_def) #> snd)) ctxt
+      val bodyb = (Binding.name id, NoSyn)
+      val bodyb_def = ( (Binding.name (id ^ "_def"), [])
+                      ,  Syntax.check_term ctxt (Const (@{const_name mk_ifun_body}, dummyT)
+                           $ inpt $ outt $ preb_term $ postb_term))
+  in 
+    (Local_Theory.define (bodyb, bodyb_def) #> snd) ppctxt
   end;
 
 val inps_parser = Parse.enum1 "and" (Parse.short_ident -- (@{keyword "::"} |-- Parse.term));
@@ -44,21 +78,24 @@ val cmlifun_parser = Parse.short_ident
                   -- ((Parse.command_name "pre" |-- Parse.term)
                       -- (@{keyword "post"} |-- Parse.term));
 
-
-Parse.short_ident -- (Parse.$$$ "pre");
-
 Outer_Syntax.local_theory  @{command_spec "cmlifun"} 
 "Implicit CML function" 
 (cmlifun_parser >> mk_fun) 
+
 *}
 
-cmlifun mythang 
-  inps x :: "@nat" 
-  outs y :: "@nat"
-  pre "forall x : @nat @ &x > 5" 
-  post "1 + 1"
+cmlifun divide 
+  inps x :: "@nat" and y :: "@nat"
+  outs z :: "@nat"
+  pre "&y > 0" 
+  post "&z = floor (&x / &y)"
 
-thm inp_mythang_def
+thm "pre_divide_def"
+thm "post_divide_def"
+
+lemma "((5,2),2) \<in> divide"
+  apply (simp add:divide_def mk_ifun_body_def evalp)
+  sledgehammer
 
 end
 
